src/typechecker/FStar.TypeChecker.Util.fsti
@@ -139,7 +139,7 @@ val short_circuit_head: term -> bool
 val maybe_add_implicit_binders: env -> binders -> binders
 val fvar_const: env -> lident -> term
 val mk_toplevel_definition: env -> lident -> term -> sigelt * term
-val reify_body: env -> steps -> term -> term
+val norm_reify: env -> steps -> term -> term
 val remove_reify: term -> term
 
 //decorating terms with monadic operators
